Protocols/PB/Safety.v
@@ -1,0 +1,115 @@
+From Coq Require Import List Bool Lia PeanoNat ListSet Permutation RelationClasses.
+From Coq Require ssrbool ssreflect.
+Import (coercions) ssrbool.
+Import ssreflect.SsrSyntax.
+From ABCProtocol.Protocols.PB Require Export Invariant.
+
+From RecordUpdate Require Import RecordUpdate.
+From stdpp Require Import tactics. (* anyway *)
+
+Module PBSafety (A : NetAddr) (R : PBTag) (Sn : Signable) (V : Value Sn) (Pf : PBProof Sn) (VBFT : ValueBFT A R Sn V Pf) 
+  (BTh : ClassicByzThreshold A) (BSett : RestrictedByzSetting A BTh)
+  (TSS0 : ThresholdSignatureSchemePrim A Sn with Definition thres := BTh.t0) (* ! *)
+  (TSS : ThresholdSignatureScheme A Sn with Module TSSPrim := TSS0)
+  (PBDT : PBDataTypes A R Sn V Pf TSS).
+
+Import A R V Pf VBFT BTh BSett TSS PBDT.
+Import ssrbool. (* anyway *)
+
+Module Export PBInv := PBInvariant A R Sn V Pf VBFT BTh BSett TSS0 TSS PBDT.
+
+Set Implicit Arguments. (* anyway *)
+
+Fact id_coh_always_holds : always_holds id_coh.
+Proof. intros w Hw. induction Hw; eauto using id_coh_is_invariant. hnf. intros. reflexivity. Qed.
+
+Fact state_invariants_always_holds : always_holds (lift_state_inv node_state_invariants).
+Proof.
+  intros w Hw. induction Hw; eauto using state_invariants.
+  constructor; hnf; unfold initWorld, initState; simpl; intros; hnf in *; try eqsolve.
+  - constructor.
+  - pose proof th_output_gt_0. lia.
+Qed.
+
+Fact l2h_invariants_always_holds : always_holds (lift_node_inv node_psent_l2h_invariants).
+Proof.
+  eapply is_invariant_reachable_step_under_closed.
+  1: hnf; intros ?????; apply l2h_invariants.
+  2: apply id_coh_always_holds.
+  hnf. intros. constructor; hnf; try discriminate; try contradiction.
+Qed.
+
+Fact h2l_invariants_always_holds : always_holds (lift_pkt_inv node_psent_h2l_invariants_nonbyz).
+Proof.
+  eapply is_invariant_reachable_step_under_closed.
+  1: hnf; intros ?????; apply h2l_invariants.
+  2: apply id_coh_always_holds.
+  hnf. intros. constructor; hnf; try discriminate; try contradiction.
+Qed.
+
+(* useful *)
+Ltac saturate :=
+  let Hcoh := fresh "Hcoh" in
+  let Hst := fresh "Hst" in
+  let Hl2h := fresh "Hl2h" in
+  let Hh2l := fresh "Hh2l" in
+  (* let Hh2lbyz := fresh "Hh2lbyz" in *)
+  match goal with
+    H : reachable ?w |- _ => 
+    pose proof (id_coh_always_holds H) as Hcoh;
+    pose proof (state_invariants_always_holds H) as Hst;
+    pose proof (l2h_invariants_always_holds H) as Hl2h;
+    pose proof (h2l_invariants_always_holds H) as Hh2l
+    (* pose proof (proj2 h2l_invariants _ H) as Hh2lbyz *)
+  end.
+
+(* TODO how to state uniqueness? *)
+
+Definition node_in_counter w : Prop :=
+  forall n src r,
+    In src (map fst ((w @ n).(counter) r)) ->
+    In (src, light_sign (r, (value_bft n r).1) (lightkey_map src)) ((w @ n).(counter) r).
+
+(* also implies external validity *)
+Definition output_ok w : Prop :=
+  forall n r cs, is_byz n = false -> (w @ n).(output) r = Some cs ->
+    let: v := (value_bft n r).1 in
+    ex_validate r v (value_bft n r).2 /\ combined_verify (r, v) cs.
+
+Lemma node_in_counter_always_holds : always_holds node_in_counter.
+Proof.
+  hnf. intros w Hr. saturate.
+  hnf. intros n ? r ((src & lsig) & <- & Hin)%in_map_iff. simpl.
+  pick counter_ok as_ H1 by_ (pose proof (Hst n) as []). pose proof Hin as ->%H1%lightkey_correct.
+  now rewrite Hcoh in Hin.
+Qed.
+
+Lemma output_ok_always_holds : always_holds output_ok.
+Proof.
+  hnf. intros w Hr. saturate.
+  hnf. intros.
+  (* basic *)
+  pick output_some as_ H1 by_ (pose proof (Hst n) as []). specialize (H1 r). isSome_rewrite. saturate_assumptions.
+  pick from_nodup as_ Hnodup by_ (pose proof (Hst n) as []). specialize (Hnodup r).
+  split.
+  - apply at_least_one_nonfaulty in Hnodup.
+    2: rewrite map_length, H1; unfold th_output; pose proof N_minus_2t0_gt_0; lia.
+    destruct Hnodup as (? & Hnonbyz_n1 & ((n1 & lsig1) & <- & Hin)%in_map_iff). simpl in Hnonbyz_n1.
+    (* in counter <-- EchoMsg recv *)
+    pick echomsg_recv_l2h as_ H2 by_ (pose proof (Hl2h _ H) as []). apply H2 in Hin. rewrite Hcoh in Hin.
+    (* <-- echoed *)
+    pick echomsg_sent_h2l as_ H3 by_ (pose proof (Hh2l _ Hin) as []). saturate_assumptions.
+    destruct (echoed (w @ n1) (n, r)) as [ (v, pf) | ] eqn:E; try contradiction. subst lsig1.
+    (* <-- InitMsg recv *)
+    pick initmsg_recv_l2h as_ H4 by_ (pose proof (Hl2h _ Hnonbyz_n1) as []). saturate_assumptions!. rewrite Hcoh in H4.
+    (* <-- sent *)
+    pick initmsg_sent_h2l as_ H5 by_ (pose proof (Hh2l _ H4) as []). saturate_assumptions. destruct H5 as (_ & ->). simpl.
+    (* <-- validated *)
+    pick echoed_ex_valid as_ H6 by_ (pose proof (Hst n1) as []). now saturate_assumptions!.
+  - apply combine_correct.
+    eexists. split; [ apply Hnodup | ]. split; [ rewrite map_length, H1; reflexivity | ].
+    pick output_is_delivery_cert as_ H2 by_ (pose proof (Hst n) as []). apply H2 in H0. subst cs. unfold delivery_cert. f_equal.
+    pick counter_ok as_ H3 by_ (pose proof (Hst n) as []). fold (counter_ok (w @ n)) in H3. rewrite counter_ok_alt in H3. rewrite H3 at 1. now rewrite map_map, Hcoh.
+Qed.
+
+End PBSafety.
